Prove init of Stackingproof

backend/LinearC.v
@@ -10,6 +10,273 @@ Set Implicit Arguments.
 
 
 
+Fixpoint fill_arguments (ls0: locset) (args: list val) (locs: list (rpair loc)): option locset :=
+  match args, locs with
+  | [], [] => Some ls0
+  | arg :: args, loc :: locs =>
+    match fill_arguments ls0 args locs with
+    | Some ls1 =>
+      match loc with
+      | One loc => Some (Locmap.set loc arg ls1)
+      | Twolong hi lo => Some (Locmap.set lo arg.(Val.loword) (Locmap.set hi arg.(Val.hiword) ls1))
+      end
+    | None => None
+    end
+  | _, _ => None
+  end
+.
+
+Local Opaque Z.mul Z.add.
+Local Opaque list_nth_z.
+
+Lemma chunk_type_chunk
+      ty
+  :
+    (type_of_chunk (chunk_of_type ty)) = ty
+.
+Proof.
+  destruct ty; ss.
+Qed.
+
+Print Loc.notin.
+Print Loc.norepet.
+Print Loc.no_overlap.
+
+Lemma Loc_cons_right_disjoint
+      xs0 xs1
+      (DISJ: Loc.disjoint xs0 xs1)
+      x
+      (NOTIN: Loc.notin x xs0)
+  :
+    <<DISJ: Loc.disjoint xs0 (x :: xs1)>>
+.
+Proof.
+  ii; ss.
+  des; ss; clarify; eauto.
+  apply Loc.diff_sym.
+  eapply Loc.in_notin_diff; eauto.
+Qed.
+
+Lemma loc_arguments_norepet_aux
+      tys (ir fr ofs: Z)
+      locs
+      (LOCS: (regs_of_rpairs (loc_arguments_64 tys ir fr ofs)) = locs)
+  :
+    (<<NOREP: Loc.norepet locs>>)
+    /\
+    (<<NOTINIR: Loc.disjoint (map R (List.firstn ir.(Z.to_nat) int_param_regs)) locs>>)
+    /\
+    (<<NOTINFR: Loc.disjoint (map R (List.firstn fr.(Z.to_nat) float_param_regs)) locs>>)
+.
+Proof.
+  ginduction tys; ii; ss; clarify.
+  { esplits; eauto.
+    - econs; eauto.
+    - ii; ss.
+    - ii; ss.
+  }
+  des_ifs; ss.
+  -
+    (* rewrite Z.add_comm in *; ss. *)
+    (* specialize (IHtys (1 + ir)%nat fr ofs _ eq_refl); des; ss. *)
+    specialize (IHtys (ir + 1) fr ofs _ eq_refl); des; ss.
+    esplits; eauto.
+    + econs; eauto.
+      eapply Loc.disjoint_notin; try apply NOTINIR.
+      admit "easy".
+    + eapply Loc_cons_right_disjoint; eauto.
+      { admit "easy". }
+      { admit "easy". }
+    + eapply Loc_cons_right_disjoint; eauto.
+      { admit "easy". }
+  - specialize (IHtys ir fr (ofs + 2) _ eq_refl); des; ss.
+    esplits; eauto.
+    + econs; eauto.
+      admit "easy".
+    + eapply Loc_cons_right_disjoint; eauto.
+      admit "easy".
+    + eapply Loc_cons_right_disjoint; eauto.
+      admit "easy".
+  - admit "ditto".
+  - admit "ditto".
+  - admit "ditto".
+  - admit "ditto".
+  - admit "ditto".
+  - admit "ditto".
+  - admit "ditto".
+  - admit "ditto".
+  - admit "ditto".
+  - admit "ditto".
+Qed.
+
+Lemma loc_arguments_norepet
+      sg
+  :
+    Loc.norepet (regs_of_rpairs (loc_arguments sg))
+.
+Proof.
+  unfold loc_arguments. des_ifs.
+  generalize (loc_arguments_norepet_aux (sig_args sg) 0 0 0). i. specialize (H _ eq_refl). des.
+  ss.
+Qed.
+
+Lemma Val_hiword_spec
+      vhi vlo
+      (DEFINED: (Val.longofwords vhi vlo) <> Vundef)
+  :
+    <<EQ: (Val.hiword (Val.longofwords vhi vlo)) = vhi>>
+.
+Proof.
+  u.
+  unfold Val.longofwords, Val.hiword. des_ifs; ss; eauto.
+  rewrite Int64.hi_ofwords. ss.
+Qed.
+
+Lemma Val_loword_spec
+      vhi vlo
+      (DEFINED: (Val.longofwords vhi vlo) <> Vundef)
+  :
+    <<EQ: (Val.loword (Val.longofwords vhi vlo)) = vlo>>
+.
+Proof.
+  u.
+  unfold Val.longofwords, Val.loword. des_ifs; ss; eauto.
+  rewrite Int64.lo_ofwords. ss.
+Qed.
+
+Ltac _locmap_tac :=
+  try (rewrite Locmap.gss; ss; []);
+  try (rewrite Locmap.gso; ss);
+  try match goal with
+      | [H: Loc.notin _ (_ :: _) |- _] => inv H
+      | [H: Loc.norepet (_ :: _) |- _] => inv H
+      | [ |- Loc.diff _ _] => by (eapply Loc.in_notin_diff; eauto)
+      | [H: Loc.diff ?A ?B |- Loc.diff ?B ?A] => apply Loc.diff_sym; assumption
+      end;
+  des_safe;
+  idtac
+.
+Local Opaque Loc.diff.
+Ltac locmap_tac := repeat _locmap_tac.
+
+Lemma fill_arguments_spec
+      (rs: regset) m sg vs ls
+      sp
+      (RSP: (rs RSP) = Vptr sp Ptrofs.zero true)
+      (EXT: extcall_arguments rs m sg vs)
+      (FILL: fill_arguments (Locmap.init Vundef) vs (loc_arguments sg) = Some ls)
+      (SZBOUND: size_arguments sg <= Ptrofs.max_unsigned / 4)
+  :
+    (<<SPEC: forall
+        ofs ty
+      ,
+        (<<INSIDE: forall (IN: In (S Outgoing ofs ty) (regs_of_rpairs (loc_arguments sg))),
+          (<<LOAD: Mem.load (chunk_of_type ty) m sp (4 * ofs) = Some (ls (S Outgoing ofs ty))>>)
+            \/ (<<UNDEF: ls (S Outgoing ofs ty) = Vundef>>)>>)
+        /\
+        (<<OUTSIDE: forall (OUT: (* Loc.notin *) ~ In (S Outgoing ofs ty) (regs_of_rpairs (loc_arguments sg))),
+            (<<UNDEF: (ls (S Outgoing ofs ty)) = Vundef>>)>>)>>)
+.
+Proof.
+  unfold extcall_arguments in *.
+  assert(BDD: forall ofs ty,
+        In (S Outgoing ofs ty) (regs_of_rpairs (loc_arguments sg)) ->
+        0 <= ofs /\ (typealign ty | ofs) /\
+        ofs + typesize ty <= Ptrofs.max_unsigned/4).
+  { i.
+    generalize (loc_arguments_acceptable_2 sg (S Outgoing ofs ty)); eauto. intro ACCP. special ACCP; ss. des.
+    esplits; ss; try xomega.
+    etransitivity; eauto.
+    generalize (loc_arguments_bounded sg); eauto.
+  }
+  assert(NOREPT: Loc.norepet (regs_of_rpairs (loc_arguments sg))).
+  { apply loc_arguments_norepet. }
+  abstr (loc_arguments sg) locs. clears sg. clear sg.
+  ginduction locs; ii; ss.
+  { split; ii; ss. destruct vs; ss. clarify. }
+  split; ii; ss.
+  {
+    assert(OFS: 0 <= 4 * ofs <= Ptrofs.max_unsigned).
+    { specialize (BDD ofs ty).
+      special BDD.
+      { ss. }
+      des_safe.
+      generalize (typesize_pos ty). i.
+      split; try xomega.
+      assert((4 * (Ptrofs.max_unsigned/4)) <= Ptrofs.max_unsigned).
+      { eapply Z_mult_div_ge. xomega. }
+      etransitivity; eauto.
+      eapply Z.mul_le_mono_pos_l with (p:=4) (n:=ofs); try xomega.
+    }
+    apply in_app_or in IN.
+    inv EXT. ss. des_ifs_safe.
+    rename l into ls0.
+    hexploit IHlocs; eauto.
+    { ii. eapply BDD. apply in_app_iff. right. ss. }
+    { admit "easy". }
+    i; des_safe. specialize (H ofs ty). des_safe.
+    des; cycle 1.
+    - special INSIDE; ss.
+      des; ss; cycle 1.
+      + right.
+        des_ifs; ss; locmap_tac.
+      + left.
+        des_ifs; ss; locmap_tac.
+    - inv H1; ss.
+      + des; ss; clarify; locmap_tac.
+        inv H. left.
+        unfold Mem.loadv, Val.offset_ptr in *. des_ifs.
+        rewrite Ptrofs.add_zero_l in *. rewrite Z.add_0_l in *. rewrite Ptrofs.unsigned_repr in *; ss.
+        rewrite Val.load_result_same; ss. rewrite <- chunk_type_chunk. eapply Mem.load_type; eauto.
+      + destruct (classic ((Val.longofwords vhi vlo) = Vundef)) eqn:T; clear T.
+        * rewrite e in *. right.
+          des; ss; clarify; locmap_tac.
+          admit "easy".
+          admit "easy".
+        * rewrite Val_hiword_spec in *; ss.
+          rewrite Val_loword_spec in *; ss.
+          clarify.
+          des; ss; clarify; locmap_tac.
+          { left.
+            inv H. ss.
+            unfold Mem.loadv, Val.offset_ptr in *. des_ifs.
+            rewrite Ptrofs.add_zero_l in *. rewrite Z.add_0_l in *. rewrite Ptrofs.unsigned_repr in *; ss.
+            rewrite Val.load_result_same; ss. rewrite <- chunk_type_chunk. eapply Mem.load_type; eauto.
+          }
+          { left.
+            inv H0. ss.
+            unfold Mem.loadv, Val.offset_ptr in *. des_ifs.
+            rewrite Ptrofs.add_zero_l in *. rewrite Z.add_0_l in *. rewrite Ptrofs.unsigned_repr in *; ss.
+            rewrite Val.load_result_same; ss. rewrite <- chunk_type_chunk. eapply Mem.load_type; eauto.
+          }
+  }
+  {
+    destruct vs; ss. inv EXT.
+    des_ifs_safe; ss.
+    hexploit IHlocs; eauto.
+    { ii. eapply BDD. apply in_app_iff. right. ss. }
+    { admit "easy". }
+    i; des. specialize (H ofs ty). des.
+    des_ifs; ss.
+    - rename r into rrr.
+      apply not_or_and in OUT. des.
+      destruct (classic (Loc.diff rrr (S Outgoing ofs ty))).
+      + locmap_tac. erewrite OUTSIDE; eauto.
+      + unfold Locmap.set. des_ifs.
+    - apply not_or_and in OUT. des.
+      apply not_or_and in OUT0. des.
+      destruct (classic (Loc.diff rlo (S Outgoing ofs ty))).
+      {
+        destruct (classic (Loc.diff rhi (S Outgoing ofs ty))).
+        { locmap_tac. erewrite OUTSIDE; eauto. }
+        unfold Locmap.set. des_ifs.
+      }
+      unfold Locmap.set. des_ifs.
+  }
+Qed.
+
+
+
 Section NEWSTEP.
 
 Variable ge: genv.
@@ -254,18 +521,6 @@ Section MODSEM.
   (*         if Mem.loadv  *)
   (*       else Vundef *)
   (* . *)
-
-  Fixpoint fill_arguments (ls0: locset) (args: list val) (locs: list (rpair loc)): option locset :=
-    match args, locs with
-    | [], [] => Some ls0
-    | arg :: args, loc :: locs =>
-      match loc with
-      | One loc => Some (Locmap.set loc arg ls0)
-      | Twolong hi lo => Some (Locmap.set lo arg.(Val.loword) (Locmap.set hi arg.(Val.hiword) ls0))
-      end
-    | _, _ => None
-    end
-  .
 
   Inductive initial_frame (rs_arg: regset) (m_arg: mem)
     : state -> Prop :=
